src/Init/Data/String/Lemmas/Basic.lean
@@ -41,7 +41,7 @@ theorem singleton_ne_empty {c : Char} : singleton c ≠ "" := by
 
 @[simp]
 theorem Slice.Pos.toCopy_inj {s : Slice} {p₁ p₂ : s.Pos} : p₁.toCopy = p₂.toCopy ↔ p₁ = p₂ := by
-  simp [Pos.ext_iff, Pos.ext_iff]
+  simp [String.Pos.ext_iff, Pos.ext_iff]
 
 @[simp]
 theorem Pos.startPos_le {s : String} (p : s.Pos) : s.startPos ≤ p := by
